Update generated Lean code (#5)
* Update generated Lean code

* `AddEquivalence.lean`: update code

* `Push0Equivalence.lean`: update code

* Update generated code to latest summaries

EvmEquivalence/Equivalence/Push0Equivalence.lean
@@ -45,44 +45,44 @@ def push0LHS
   {_Gen8 : SortCallGasCell}
   {_Gen9 : SortStaticCell}: SortGeneratedTopCell :=
   { kevm := {
-    k := { val := SortK.kseq ((@inj SortInternalOp SortKItem) (SortInternalOp.«#next[_]_EVM_InternalOp_MaybeOpCode» ((@inj SortPushOp SortMaybeOpCode) SortPushOp.PUSHZERO_EVM_PushOp))) K_CELL },
-    exitCode := _Gen22,
-    mode := _Gen23,
-    schedule := { val := SCHEDULE_CELL },
-    useGas := { val := USEGAS_CELL },
-    ethereum := {
-      evm := {
-        output := _Gen11,
-        statusCode := _Gen12,
-        callStack := _Gen13,
-        interimStates := _Gen14,
-        touchedAccounts := _Gen15,
-        callState := {
-          program := _Gen0,
-          jumpDests := _Gen1,
-          id := _Gen2,
-          caller := _Gen3,
-          callData := _Gen4,
-          callValue := _Gen5,
-          wordStack := { val := WS },
-          localMem := _Gen6,
-          pc := { val := PC_CELL },
-          gas := { val := (@inj SortInt SortGas) GAS_CELL },
-          memoryUsed := _Gen7,
-          callGas := _Gen8,
-          static := _Gen9,
-          callDepth := _Gen10 },
-        versionedHashes := _Gen16,
-        substate := _Gen17,
-        gasPrice := _Gen18,
-        origin := _Gen19,
-        blockhashes := _Gen20,
-        block := _Gen21 },
-      network := _DotVar2 } },
+      k := { val := SortK.kseq ((@inj SortInternalOp SortKItem) (SortInternalOp.«#next[_]_EVM_InternalOp_MaybeOpCode» ((@inj SortPushOp SortMaybeOpCode) SortPushOp.PUSHZERO_EVM_PushOp))) K_CELL },
+      exitCode := _Gen22,
+      mode := _Gen23,
+      schedule := { val := SCHEDULE_CELL },
+      useGas := { val := USEGAS_CELL },
+      ethereum := {
+        evm := {
+          output := _Gen11,
+          statusCode := _Gen12,
+          callStack := _Gen13,
+          interimStates := _Gen14,
+          touchedAccounts := _Gen15,
+          callState := {
+            program := _Gen0,
+            jumpDests := _Gen1,
+            id := _Gen2,
+            caller := _Gen3,
+            callData := _Gen4,
+            callValue := _Gen5,
+            wordStack := { val := WS },
+            localMem := _Gen6,
+            pc := { val := PC_CELL },
+            gas := { val := (@inj SortInt SortGas) GAS_CELL },
+            memoryUsed := _Gen7,
+            callGas := _Gen8,
+            static := _Gen9,
+            callDepth := _Gen10 },
+          versionedHashes := _Gen16,
+          substate := _Gen17,
+          gasPrice := _Gen18,
+          origin := _Gen19,
+          blockhashes := _Gen20,
+          block := _Gen21 },
+        network := _DotVar2 } },
     generatedCounter := _DotVar0 }
 
 def push0RHS
-  {_Val10 _Val8 : SortInt}
+  {_Val11 _Val13 : SortInt}
   {K_CELL : SortK}
   {SCHEDULE_CELL : SortSchedule}
   {WS : SortWordStack}
@@ -113,47 +113,47 @@ def push0RHS
   {_Gen8 : SortCallGasCell}
   {_Gen9 : SortStaticCell}: SortGeneratedTopCell :=
   { kevm := {
-    k := { val := K_CELL },
-    exitCode := _Gen22,
-    mode := _Gen23,
-    schedule := { val := SCHEDULE_CELL },
-    useGas := { val := true },
-    ethereum := {
-      evm := {
-        output := _Gen11,
-        statusCode := _Gen12,
-        callStack := _Gen13,
-        interimStates := _Gen14,
-        touchedAccounts := _Gen15,
-        callState := {
-          program := _Gen0,
-          jumpDests := _Gen1,
-          id := _Gen2,
-          caller := _Gen3,
-          callData := _Gen4,
-          callValue := _Gen5,
-          wordStack := { val := SortWordStack.«_:__EVM-TYPES_WordStack_Int_WordStack» 0 WS },
-          localMem := _Gen6,
-          pc := { val := _Val8 },
-          gas := { val := (@inj SortInt SortGas) _Val10 },
-          memoryUsed := _Gen7,
-          callGas := _Gen8,
-          static := _Gen9,
-          callDepth := _Gen10 },
-        versionedHashes := _Gen16,
-        substate := _Gen17,
-        gasPrice := _Gen18,
-        origin := _Gen19,
-        blockhashes := _Gen20,
-        block := _Gen21 },
-      network := _DotVar2 } },
+      k := { val := K_CELL },
+      exitCode := _Gen22,
+      mode := _Gen23,
+      schedule := { val := SCHEDULE_CELL },
+      useGas := { val := true },
+      ethereum := {
+        evm := {
+          output := _Gen11,
+          statusCode := _Gen12,
+          callStack := _Gen13,
+          interimStates := _Gen14,
+          touchedAccounts := _Gen15,
+          callState := {
+            program := _Gen0,
+            jumpDests := _Gen1,
+            id := _Gen2,
+            caller := _Gen3,
+            callData := _Gen4,
+            callValue := _Gen5,
+            wordStack := { val := SortWordStack.«_:__EVM-TYPES_WordStack_Int_WordStack» 0 WS },
+            localMem := _Gen6,
+            pc := { val := _Val11 },
+            gas := { val := (@inj SortInt SortGas) _Val13 },
+            memoryUsed := _Gen7,
+            callGas := _Gen8,
+            static := _Gen9,
+            callDepth := _Gen10 },
+          versionedHashes := _Gen16,
+          substate := _Gen17,
+          gasPrice := _Gen18,
+          origin := _Gen19,
+          blockhashes := _Gen20,
+          block := _Gen21 },
+        network := _DotVar2 } },
     generatedCounter := _DotVar0 }
 
 theorem rw_push0LHS_push0RHS
-  {GAS_CELL PC_CELL _Val0 _Val10 _Val3 _Val8 _Val9 : SortInt}
+  {GAS_CELL PC_CELL _Val0 _Val11 _Val12 _Val13 _Val3 _Val6 : SortInt}
   {K_CELL : SortK}
   {SCHEDULE_CELL : SortSchedule}
-  {USEGAS_CELL _Val1 _Val2 _Val4 _Val5 _Val6 _Val7 : SortBool}
+  {USEGAS_CELL _Val1 _Val10 _Val2 _Val4 _Val5 _Val7 _Val8 _Val9 : SortBool}
   {WS : SortWordStack}
   {_DotVar0 : SortGeneratedCounterCell}
   {_DotVar2 : SortNetworkCell}
@@ -181,22 +181,25 @@ theorem rw_push0LHS_push0RHS
   {_Gen7 : SortMemoryUsedCell}
   {_Gen8 : SortCallGasCell}
   {_Gen9 : SortStaticCell}
-  (defn_Val0 : sizeWordStackAux WS 0 = some _Val0)
-  (defn_Val1 : «_<Int_» _Val0 0 = some _Val1)
-  (defn_Val2 : notBool_ _Val1 = some _Val2)
+  (defn_Val0 : «_<_>_SCHEDULE_Int_ScheduleConst_Schedule» SortScheduleConst.Gbase_SCHEDULE_ScheduleConst SCHEDULE_CELL = some _Val0)
+  (defn_Val1 : «_<=Int_» _Val0 GAS_CELL = some _Val1)
+  (defn_Val2 : _andBool_ USEGAS_CELL _Val1 = some _Val2)
   (defn_Val3 : sizeWordStackAux WS 0 = some _Val3)
-  (defn_Val4 : «_<Int_» 1023 _Val3 = some _Val4)
+  (defn_Val4 : «_<Int_» _Val3 0 = some _Val4)
   (defn_Val5 : notBool_ _Val4 = some _Val5)
-  (defn_Val6 : _andBool_ _Val2 _Val5 = some _Val6)
-  (defn_Val7 : _andBool_ USEGAS_CELL _Val6 = some _Val7)
-  (defn_Val8 : «_+Int_» PC_CELL 1 = some _Val8)
-  (defn_Val9 : «_<_>_SCHEDULE_Int_ScheduleConst_Schedule» SortScheduleConst.Gbase_SCHEDULE_ScheduleConst SCHEDULE_CELL = some _Val9)
-  (defn_Val10 : «_-Int_» GAS_CELL _Val9 = some _Val10)
-  (req : _Val7 = true):
+  (defn_Val6 : sizeWordStackAux WS 0 = some _Val6)
+  (defn_Val7 : «_<Int_» 1023 _Val6 = some _Val7)
+  (defn_Val8 : notBool_ _Val7 = some _Val8)
+  (defn_Val9 : _andBool_ _Val5 _Val8 = some _Val9)
+  (defn_Val10 : _andBool_ _Val2 _Val9 = some _Val10)
+  (defn_Val11 : «_+Int_» PC_CELL 1 = some _Val11)
+  (defn_Val12 : «_<_>_SCHEDULE_Int_ScheduleConst_Schedule» SortScheduleConst.Gbase_SCHEDULE_ScheduleConst SCHEDULE_CELL = some _Val12)
+  (defn_Val13 : «_-Int_» GAS_CELL _Val12 = some _Val13)
+  (req : _Val10 = true) :
   Rewrites
   (@push0LHS GAS_CELL PC_CELL K_CELL SCHEDULE_CELL USEGAS_CELL WS _DotVar0 _DotVar2 _Gen0 _Gen1 _Gen10 _Gen11 _Gen12 _Gen13 _Gen14 _Gen15 _Gen16 _Gen17 _Gen18 _Gen19 _Gen2 _Gen20 _Gen21 _Gen22 _Gen23 _Gen3 _Gen4 _Gen5 _Gen6 _Gen7 _Gen8 _Gen9)
-  (@push0RHS _Val10 _Val8 K_CELL SCHEDULE_CELL WS _DotVar0 _DotVar2 _Gen0 _Gen1 _Gen10 _Gen11 _Gen12 _Gen13 _Gen14 _Gen15 _Gen16 _Gen17 _Gen18 _Gen19 _Gen2 _Gen20 _Gen21 _Gen22 _Gen23 _Gen3 _Gen4 _Gen5 _Gen6 _Gen7 _Gen8 _Gen9) :=
-  by apply Rewrites.SUMMARY_PUSHZERO_0_SPEC_BASIC_BLOCK_11_TO_9 <;> try assumption
+  (@push0RHS _Val11 _Val13 K_CELL SCHEDULE_CELL WS _DotVar0 _DotVar2 _Gen0 _Gen1 _Gen10 _Gen11 _Gen12 _Gen13 _Gen14 _Gen15 _Gen16 _Gen17 _Gen18 _Gen19 _Gen2 _Gen20 _Gen21 _Gen22 _Gen23 _Gen3 _Gen4 _Gen5 _Gen6 _Gen7 _Gen8 _Gen9) :=
+  by apply Rewrites.SUMMARY_PUSHZERO_0_SPEC_BASIC_BLOCK_25_TO_24 <;> try assumption
      all_goals simp_all [notBool_def, andBool_def]
 
 theorem push0_prestate_equiv
@@ -243,7 +246,7 @@ theorem push0_prestate_equiv
 
 theorem push0_poststate_equiv
   (PC_CELL : SortInt)
-  {_Val10 _Val8 : SortInt}
+  {_Val11 _Val13 : SortInt}
   {K_CELL : SortK}
   {SCHEDULE_CELL : SortSchedule}
   {WS : SortWordStack}
@@ -274,21 +277,21 @@ theorem push0_poststate_equiv
   {_Gen8 : SortCallGasCell}
   {_Gen9 : SortStaticCell}
   {symState : EVM.State}
-  (defn_Val8 : «_+Int_» PC_CELL 1 = some _Val8):
-  stateMap symState (@push0RHS _Val10 _Val8 K_CELL SCHEDULE_CELL WS _DotVar0 _DotVar2 _Gen0 _Gen1 _Gen10 _Gen11 _Gen12 _Gen13 _Gen14 _Gen15 _Gen16 _Gen17 _Gen18 _Gen19 _Gen2 _Gen20 _Gen21 _Gen22 _Gen23 _Gen3 _Gen4 _Gen5 _Gen6 _Gen7 _Gen8 _Gen9) =
+  (defn_Val11 : «_+Int_» PC_CELL 1 = some _Val11):
+  stateMap symState (@push0RHS _Val11 _Val13 K_CELL SCHEDULE_CELL WS _DotVar0 _DotVar2 _Gen0 _Gen1 _Gen10 _Gen11 _Gen12 _Gen13 _Gen14 _Gen15 _Gen16 _Gen17 _Gen18 _Gen19 _Gen2 _Gen20 _Gen21 _Gen22 _Gen23 _Gen3 _Gen4 _Gen5 _Gen6 _Gen7 _Gen8 _Gen9) =
   {symState with
     stack := .ofNat 0 :: wordStackMap WS
     pc := intMap («_+Int'_» PC_CELL 1)
-    gasAvailable := intMap _Val10
+    gasAvailable := intMap _Val13
     executionEnv := {symState.executionEnv with code := _Gen0.val}
     returnData := _Gen11.val
     } := by aesop (add simp [«_+Int'_»])
 
 theorem step_push0_equiv
-  {GAS_CELL PC_CELL _Val0 _Val10 _Val3 _Val8 _Val9 : SortInt}
+  {GAS_CELL PC_CELL _Val0 _Val11 _Val12 _Val13 _Val3 _Val6 : SortInt}
   {K_CELL : SortK}
   {SCHEDULE_CELL : SortSchedule}
-  {USEGAS_CELL _Val1 _Val2 _Val4 _Val5 _Val6 _Val7 : SortBool}
+  {USEGAS_CELL _Val1 _Val10 _Val2 _Val4 _Val5 _Val7 _Val8 _Val9 : SortBool}
   {WS : SortWordStack}
   {_DotVar0 : SortGeneratedCounterCell}
   {_DotVar2 : SortNetworkCell}
@@ -316,19 +319,22 @@ theorem step_push0_equiv
   {_Gen7 : SortMemoryUsedCell}
   {_Gen8 : SortCallGasCell}
   {_Gen9 : SortStaticCell}
-  {symState : EVM.State}
-  (defn_Val0 : sizeWordStackAux WS 0 = some _Val0)
-  (defn_Val1 : «_<Int_» _Val0 0 = some _Val1)
-  (defn_Val2 : notBool_ _Val1 = some _Val2)
+  (defn_Val0 : «_<_>_SCHEDULE_Int_ScheduleConst_Schedule» SortScheduleConst.Gbase_SCHEDULE_ScheduleConst SCHEDULE_CELL = some _Val0)
+  (defn_Val1 : «_<=Int_» _Val0 GAS_CELL = some _Val1)
+  /- (defn_Val2 : _andBool_ USEGAS_CELL _Val1 = some _Val2) -/
   (defn_Val3 : sizeWordStackAux WS 0 = some _Val3)
-  (defn_Val4 : «_<Int_» 1023 _Val3 = some _Val4)
-  (defn_Val5 : notBool_ _Val4 = some _Val5)
-  (defn_Val6 : _andBool_ _Val2 _Val5 = some _Val6)
-  (defn_Val7 : _andBool_ USEGAS_CELL _Val6 = some _Val7)
-  (defn_Val8 : «_+Int_» PC_CELL 1 = some _Val8)
-  (defn_Val9 : «_<_>_SCHEDULE_Int_ScheduleConst_Schedule» SortScheduleConst.Gbase_SCHEDULE_ScheduleConst SCHEDULE_CELL = some _Val9)
-  (defn_Val10 : «_-Int_» GAS_CELL _Val9 = some _Val10)
-  (req : _Val7 = true)
+  (defn_Val4 : «_<Int_» _Val3 0 = some _Val4)
+  /- (defn_Val5 : notBool_ _Val4 = some _Val5) -/
+  (defn_Val6 : sizeWordStackAux WS 0 = some _Val6)
+  (defn_Val7 : «_<Int_» 1023 _Val6 = some _Val7)
+  /- (defn_Val8 : notBool_ _Val7 = some _Val8)
+  (defn_Val9 : _andBool_ _Val5 _Val8 = some _Val9) -/
+  (defn_Val10 : _andBool_ _Val2 _Val9 = some _Val10)
+  (defn_Val11 : «_+Int_» PC_CELL 1 = some _Val11)
+  (defn_Val12 : «_<_>_SCHEDULE_Int_ScheduleConst_Schedule» SortScheduleConst.Gbase_SCHEDULE_ScheduleConst SCHEDULE_CELL = some _Val12)
+  (defn_Val13 : «_-Int_» GAS_CELL _Val12 = some _Val13)
+  (req : _Val10 = true)
+  (symState : EVM.State)
   -- needed for EVM.step
   (gas gasCost : ℕ)
   -- Necessary assumptions for equivalence
@@ -340,7 +346,7 @@ theorem step_push0_equiv
   (pcountSmall : PC_CELL + 1 < UInt256.size)
   (pcountNonneg : 0 ≤ PC_CELL):
   EVM.step_push0 gas gasCost (stateMap symState (@push0LHS GAS_CELL PC_CELL K_CELL SCHEDULE_CELL USEGAS_CELL WS _DotVar0 _DotVar2 _Gen0 _Gen1 _Gen10 _Gen11 _Gen12 _Gen13 _Gen14 _Gen15 _Gen16 _Gen17 _Gen18 _Gen19 _Gen2 _Gen20 _Gen21 _Gen22 _Gen23 _Gen3 _Gen4 _Gen5 _Gen6 _Gen7 _Gen8 _Gen9)) =
-  .ok (stateMap {symState with execLength := symState.execLength + 1} (@push0RHS _Val10 _Val8 K_CELL SCHEDULE_CELL WS _DotVar0 _DotVar2 _Gen0 _Gen1 _Gen10 _Gen11 _Gen12 _Gen13 _Gen14 _Gen15 _Gen16 _Gen17 _Gen18 _Gen19 _Gen2 _Gen20 _Gen21 _Gen22 _Gen23 _Gen3 _Gen4 _Gen5 _Gen6 _Gen7 _Gen8 _Gen9)) := by
+  .ok (stateMap {symState with execLength := symState.execLength + 1} (@push0RHS _Val11 _Val13 K_CELL SCHEDULE_CELL WS _DotVar0 _DotVar2 _Gen0 _Gen1 _Gen10 _Gen11 _Gen12 _Gen13 _Gen14 _Gen15 _Gen16 _Gen17 _Gen18 _Gen19 _Gen2 _Gen20 _Gen21 _Gen22 _Gen23 _Gen3 _Gen4 _Gen5 _Gen6 _Gen7 _Gen8 _Gen9)) := by
   rw [push0_prestate_equiv, (push0_poststate_equiv PC_CELL)]
   cases gas; contradiction
   rw [EVM.step_push0_summary] <;> try assumption
@@ -352,10 +358,10 @@ theorem step_push0_equiv
 attribute [local simp] GasConstants.Gbase
 
 theorem X_push0_equiv
-  {GAS_CELL PC_CELL _Val0 _Val10 _Val3 _Val8 _Val9 : SortInt}
+  {GAS_CELL PC_CELL _Val0 _Val11 _Val12 _Val13 _Val3 _Val6 : SortInt}
   {K_CELL : SortK}
   {SCHEDULE_CELL : SortSchedule}
-  {USEGAS_CELL _Val1 _Val2 _Val4 _Val5 _Val6 _Val7 : SortBool}
+  {USEGAS_CELL _Val1 _Val10 _Val2 _Val4 _Val5 _Val7 _Val8 _Val9 : SortBool}
   {WS : SortWordStack}
   {_DotVar0 : SortGeneratedCounterCell}
   {_DotVar2 : SortNetworkCell}
@@ -383,19 +389,22 @@ theorem X_push0_equiv
   {_Gen7 : SortMemoryUsedCell}
   {_Gen8 : SortCallGasCell}
   {_Gen9 : SortStaticCell}
-  {symState : EVM.State}
-  (defn_Val0 : sizeWordStackAux WS 0 = some _Val0)
-  (defn_Val1 : «_<Int_» _Val0 0 = some _Val1)
-  --(defn_Val2 : notBool_ _Val1 = some _Val2)
+  (defn_Val0 : «_<_>_SCHEDULE_Int_ScheduleConst_Schedule» SortScheduleConst.Gbase_SCHEDULE_ScheduleConst SCHEDULE_CELL = some _Val0)
+  (defn_Val1 : «_<=Int_» _Val0 GAS_CELL = some _Val1)
+  (defn_Val2 : _andBool_ USEGAS_CELL _Val1 = some _Val2)
   (defn_Val3 : sizeWordStackAux WS 0 = some _Val3)
-  (defn_Val4 : «_<Int_» 1023 _Val3 = some _Val4)
-  (defn_Val5 : notBool_ _Val4 = some _Val5)
-  (defn_Val6 : _andBool_ _Val2 _Val5 = some _Val6)
-  (defn_Val7 : _andBool_ USEGAS_CELL _Val6 = some _Val7)
-  (defn_Val8 : «_+Int_» PC_CELL 1 = some _Val8)
-  (defn_Val9 : «_<_>_SCHEDULE_Int_ScheduleConst_Schedule» SortScheduleConst.Gbase_SCHEDULE_ScheduleConst SCHEDULE_CELL = some _Val9)
-  (defn_Val10 : «_-Int_» GAS_CELL _Val9 = some _Val10)
-  (req : _Val7 = true)
+  (defn_Val4 : «_<Int_» _Val3 0 = some _Val4)
+  --(defn_Val5 : notBool_ _Val4 = some _Val5)
+  (defn_Val6 : sizeWordStackAux WS 0 = some _Val6)
+  (defn_Val7 : «_<Int_» 1023 _Val6 = some _Val7)
+  (defn_Val8 : notBool_ _Val7 = some _Val8)
+  (defn_Val9 : _andBool_ _Val5 _Val8 = some _Val9)
+  (defn_Val10 : _andBool_ _Val2 _Val9 = some _Val10)
+  (defn_Val11 : «_+Int_» PC_CELL 1 = some _Val11)
+  (defn_Val12 : «_<_>_SCHEDULE_Int_ScheduleConst_Schedule» SortScheduleConst.Gbase_SCHEDULE_ScheduleConst SCHEDULE_CELL = some _Val12)
+  (defn_Val13 : «_-Int_» GAS_CELL _Val12 = some _Val13)
+  (req : _Val10 = true)
+  (symState : EVM.State)
   -- Necessary assumptions for equivalence
   (cancun : SCHEDULE_CELL = .CANCUN_EVM)
   --(gasEnough : 0 < gas)
@@ -408,7 +417,7 @@ theorem X_push0_equiv
   (pcZero : PC_CELL = 0)
   (returnEmpty : _Gen11 = ⟨ByteArray.empty⟩):
   EVM.X false (UInt256.toNat (intMap GAS_CELL)) (stateMap symState (@push0LHS GAS_CELL PC_CELL K_CELL SCHEDULE_CELL USEGAS_CELL WS _DotVar0 _DotVar2 _Gen0 _Gen1 _Gen10 _Gen11 _Gen12 _Gen13 _Gen14 _Gen15 _Gen16 _Gen17 _Gen18 _Gen19 _Gen2 _Gen20 _Gen21 _Gen22 _Gen23 _Gen3 _Gen4 _Gen5 _Gen6 _Gen7 _Gen8 _Gen9)) =
-  .ok (.success (stateMap {symState with execLength := symState.execLength + 2} (@push0RHS _Val10 _Val8 K_CELL SCHEDULE_CELL WS _DotVar0 _DotVar2 _Gen0 _Gen1 _Gen10 _Gen11 _Gen12 _Gen13 _Gen14 _Gen15 _Gen16 _Gen17 _Gen18 _Gen19 _Gen2 _Gen20 _Gen21 _Gen22 _Gen23 _Gen3 _Gen4 _Gen5 _Gen6 _Gen7 _Gen8 _Gen9)) ByteArray.empty) := by
+  .ok (.success (stateMap {symState with execLength := symState.execLength + 2} (@push0RHS _Val11 _Val13 K_CELL SCHEDULE_CELL WS _DotVar0 _DotVar2 _Gen0 _Gen1 _Gen10 _Gen11 _Gen12 _Gen13 _Gen14 _Gen15 _Gen16 _Gen17 _Gen18 _Gen19 _Gen2 _Gen20 _Gen21 _Gen22 _Gen23 _Gen3 _Gen4 _Gen5 _Gen6 _Gen7 _Gen8 _Gen9)) ByteArray.empty) := by
   rw [codePush0, pcZero, push0_prestate_equiv, (push0_poststate_equiv PC_CELL)] <;> try assumption
   rw [intMap_toNat] <;> first | linarith | try assumption
   cases cgc: (UInt256.toNat (intMap GAS_CELL))
@@ -418,7 +427,8 @@ theorem X_push0_equiv
     . aesop (add simp [«_-Int_», intMap_sub_dist])
       (add safe (by rw [intMap_sub_dist])) (add safe (by linarith))
     . rw [intMap_toNat] <;> aesop (add safe (by linarith))
-    . revert defn_Val4; simp_all [sizeWordStack_def, andBool_def, notBool_def,  ltInt_def]
-      aesop (add safe (by linarith))
+    . simp [defn_Val3] at defn_Val6; subst defn_Val6
+      aesop (add simp [sizeWordStack_def, andBool_def, notBool_def,  ltInt_def])
+      (add safe (by linarith))
 
 end Push0Equivalence
